changed interp_br and continuations to allow for albitrary end result after a br

theories/iris_logrel.v
@@ -245,7 +245,7 @@ Section logrel.
 
   Notation BR := ((leibnizO val) -n> (leibnizO lholed) -n> (leibnizO (list (list value_type))) -n> iPropO Σ).
   
-  Definition interp_br_def (τs : result_type) (τl : result_type) (i : instance)
+  Definition interp_br_def (τl : result_type) (i : instance)
                        (interp_br' : BR) : BR :=
     λne (w : leibnizO val) (lh : leibnizO lholed) (τc : leibnizO (list (list value_type))),
       ((∃ j (v : list value) es, ⌜w = brV j v es⌝ ∗
@@ -255,9 +255,9 @@ Section logrel.
                                      interp_val (τs'' ++ τs') (immV v) ∗
                                      ∀ f, ↪[frame] f ∗ interp_frame τl i f -∗
                                      WP of_val (immV (drop (length τs'') v)) ++ [::AI_basic (BI_br j)] CTX S (lh_depth lh'); LH_rec vs k es lh' es'
-                                     {{ vs, (interp_val τs vs ∨ ▷ interp_br' vs lh'' (drop (S j) τc)) ∗ ∃ f, ↪[frame] f ∗ interp_frame τl i f }}))%I.
+                                     {{ vs, ((∃ τs, interp_val τs vs) ∨ ▷ interp_br' vs lh'' (drop (S j) τc)) ∗ ∃ f, ↪[frame] f ∗ interp_frame τl i f }}))%I.
 
-  Global Instance interp_br_def_contractive τs τl i : Contractive (interp_br_def τs τl i).
+  Global Instance interp_br_def_contractive τl i : Contractive (interp_br_def τl i).
   Proof.
     solve_proper_prepare.
     repeat (apply exist_ne +
@@ -269,15 +269,15 @@ Section logrel.
     solve_contractive.
   Defined.
   
-  Definition interp_br (τs : result_type) (τl : result_type) (i : instance) : BR :=
-    fixpoint (interp_br_def τs τl i).
+  Definition interp_br (τl : result_type) (i : instance) : BR :=
+    fixpoint (interp_br_def τl i).
   
-  Lemma fixpoint_interp_br_eq (τc : list (list (value_type))) (τs : result_type) (lh : lholed) (τl : result_type) (i : instance) v :
-    interp_br τs τl i v lh τc ≡ interp_br_def τs τl i (interp_br τs τl i) v lh τc.
-  Proof. exact: (fixpoint_unfold (interp_br_def τs τl i) v lh τc). Qed.
+  Lemma fixpoint_interp_br_eq (τc : list (list (value_type))) (lh : lholed) (τl : result_type) (i : instance) v :
+    interp_br τl i v lh τc ≡ interp_br_def τl i (interp_br τl i) v lh τc.
+  Proof. exact: (fixpoint_unfold (interp_br_def τl i) v lh τc). Qed.
   
   Definition interp_expression (τc : list (list (value_type))) (τs : result_type) (lh : lholed) (τl : result_type) (i : instance) (es : expr) : iProp Σ :=
-    (WP es {{ vs, (interp_val τs vs ∨ interp_br τs τl i vs lh τc) ∗ ∃ f, ↪[frame] f ∗ interp_frame τl i f }})%I.
+    (WP es {{ vs, (interp_val τs vs ∨ interp_br τl i vs lh τc) ∗ ∃ f, ↪[frame] f ∗ interp_frame τl i f }})%I.
   
   
   (* --------------------------------------------------------------------------------------- *)
@@ -311,28 +311,28 @@ Section logrel.
                                                   interp_val τs v -∗ ↪[frame] f ∗ interp_frame τl i f -∗
                                                   interp_expression τs2 lh'' (vs ++ ((of_val v) ++ es) ++ es') (interp_frame τl i)))%I.*)
 
-  Definition interp_ctx_continuation (τc : list (list (value_type))) (lh : lholed) (k : nat) (τs τl τs2 : result_type) (i : instance) : iProp Σ :=
+  Definition interp_ctx_continuation (τc : list (list (value_type))) (lh : lholed) (k : nat) (τs τl : result_type) (i : instance) : iProp Σ :=
     (∃ vs j es lh' es' lh'', ⌜get_layer lh ((lh_depth lh) - S k) = Some (vs,j,es,lh',es')⌝ ∧ ⌜lh_depth lh'' = (lh_depth lh) - S k⌝ ∧ ⌜is_Some (lh_minus lh lh'')⌝ ∧
                           (□ ∀ v f, interp_val τs v -∗ ↪[frame] f ∗ interp_frame τl i f -∗
-                                    interp_expression (drop (S k) τc) τs2 lh'' τl i (vs ++ ((of_val v) ++ es) ++ es')))%I.
+                                    ∃ τs2, interp_expression (drop (S k) τc) τs2 lh'' τl i (vs ++ ((of_val v) ++ es) ++ es')))%I.
   
-  Definition interp_ctx_continuations (τc : list (list (value_type))) (τs2 : result_type) (τl : result_type) (i : instance) : CtxR :=
-    λne lh, ([∗ list] k↦τs ∈ τc, interp_ctx_continuation τc lh k τs τl τs2 i)%I.
+  Definition interp_ctx_continuations (τc : list (list (value_type))) (τl : result_type) (i : instance) : CtxR :=
+    λne lh, ([∗ list] k↦τs ∈ τc, interp_ctx_continuation τc lh k τs τl i)%I.
 
   (* Definition interp_ctx_return (τc : list (list (value_type))) (τs2 : result_type) (τl : result_type) (i : instance) : CtxR := *)
   (*   λne lh, (□ ∀ v f, interp_val τs2 v -∗ ↪[frame] f ∗ interp_frame τl i f -∗ interp_expression_ctx τs2 lh (of_val v) τl i)%I. *)
   
-  Definition interp_ctx (τc : list (list value_type)) (τs2 : result_type) (τl : result_type) (i : instance) : CtxR :=
+  Definition interp_ctx (τc : list (list value_type)) (τl : result_type) (i : instance) : CtxR :=
     λne lh, (⌜base_is_empty lh⌝ ∗
              ⌜lholed_lengths (rev τc) lh⌝ ∗
              ⌜lholed_valid lh⌝ ∗
-             interp_ctx_continuations τc τs2 τl i lh
+             interp_ctx_continuations τc τl i lh
              (* interp_ctx_return τc τs2 τl i lh *)
             )%I.
 
-  Global Instance interp_ctx_continuations_persistent τc τs1 τs2 τl i lh : Persistent (interp_ctx_continuations τc τs2 τl i lh).
+  Global Instance interp_ctx_continuations_persistent τc τl i lh : Persistent (interp_ctx_continuations τc τl i lh).
   Proof. apply _. Qed.
-  Global Instance interp_ctx_persistent τc τs1 τs2 τl i lh : Persistent (interp_ctx τc τs2 τl i lh).
+  Global Instance interp_ctx_persistent τc τl i lh : Persistent (interp_ctx τc τl i lh).
   Proof. apply _. Qed.
 
   Notation IctxR := ((leibnizO instance) -n> (leibnizO lholed) -n> (leibnizO frame) -n> iPropO Σ).
@@ -349,7 +349,7 @@ Section logrel.
     match tf with
     | Tf τ1 τ2 => ∀ i lh, (* interp_instance_ctx τctx i lh f -∗ *)
                               interp_instance τctx i -∗
-                              interp_ctx (tc_label τctx) τ2 (tc_local τctx) i lh -∗
+                              interp_ctx (tc_label τctx) (tc_local τctx) i lh -∗
                               ∀ f vs, ↪[frame] f ∗ interp_frame (tc_local τctx) i f -∗
                                       interp_val τ1 vs -∗
                                       interp_expression (tc_label τctx) τ2 lh (tc_local τctx) i ((of_val vs) ++ es)
